Reduce parse_print to three cheats
The main one is about being able to parse one sexp followed by a
separating character (dot or space or close-paren) and have this be the
same as just parsing the sexp on its own (leaving the rest of the string
unconsumed).

The other cheats are about using that lemma for parsing some
space-separated lists of sexps.

examples/formal-languages/context-free/simpleSexpParseScript.sml
@@ -76,10 +76,20 @@ val num_to_dec_string_eq_cons = Q.store_thm("num_to_dec_string_eq_cons",
   \\ rw[] \\ res_tac \\ simp[UNHEX_HEX]);
 
 val peg_eval_list_tok_nil = Q.store_thm("peg_eval_list_tok_nil",
-  `∀ls. EVERY ($~ o P) ls ⇒
+  `∀ls. (ls = [] ∨ ¬ P(HD ls)) ⇒
    peg_eval_list G (ls, tok P a) (ls,[])`,
   rw[Once peg_eval_list,peg_eval_tok_NONE,listTheory.EVERY_MEM]
   \\ Cases_on`ls` \\ fs[]);
+
+val peg_eval_list_tok_imp_every = Q.store_thm("peg_eval_list_tok_imp_every",
+  `∀ls r z. peg_eval_list G (ls, tok P a) (r,z) ⇒
+   ∃l. ls = l ++ r ∧ EVERY P l ∧ (¬NULL r ⇒ ¬P (HD r))`,
+  Induct \\ rw[Once peg_eval_list,listTheory.NULL_EQ,peg_eval_tok_SOME]
+  \\ fs[peg_eval_tok_NONE]
+  \\ res_tac
+  \\ rpt var_eq_tac
+  \\ qexists_tac`h::l`
+  \\ rw[] \\ fs[listTheory.NULL_EQ]);
 
 (* -- *)
 
@@ -158,15 +168,24 @@ val peg_eval_valid_symbol = Q.prove(
   simp[destSXSYM_def] >> rw[] >>
   rw[Once peg_eval_cases] >> simp[peg_eval_tok_NONE]);
 
+val valid_symbol_no_spaces = Q.store_thm("valid_symbol_no_spaces",
+  `∀s. valid_symbol s ⇒ EVERY ($~ o isSpace) s`,
+  Cases_on`s` \\ rw[valid_symbol_def]
+  >- ( fs[stringTheory.isGraph_def,stringTheory.isSpace_def] )
+  \\ Induct_on`t`
+  \\ rw[]
+  >- ( fs[stringTheory.isGraph_def,stringTheory.isSpace_def] ))
+
 val peg_eval_list_num_to_dec_string_no_spaces = Q.prove(
   `peg_eval_list sexpPEG (toString n,tok isSpace ARB) (toString n,[])`,
   match_mp_tac peg_eval_list_tok_nil
   \\ assume_tac EVERY_isDigit_num_to_dec_string
   \\ fs[listTheory.EVERY_MEM] \\ rw[]
+  \\ Cases_on`toString n` \\ fs[]
   \\ fs[stringTheory.isDigit_def,stringTheory.isSpace_def]
   \\ spose_not_then strip_assume_tac
-  \\ res_tac
-  \\ DECIDE_TAC);
+  \\ first_x_assum(qspec_then`h`mp_tac)
+  \\ simp[]);
 
 val peg_eval_list_digits = Q.store_thm("peg_eval_list_digits",
   `∀s. EVERY isDigit s ⇒
@@ -303,36 +322,105 @@ val peg_eval_list_isSpace_print_sexp = Q.store_thm("peg_eval_list_isSpace_print_
   \\ simp[Once peg_eval_list]
   \\ simp[peg_eval_tok_NONE]);
 
-val peg_eval_print_sexp = Q.prove(
+val peg_eval_print_sexp_sxnt_sexp = Q.store_thm("peg_eval_print_sexp_sxnt_sexp",
+  `valid_sexp s ⇒
+   (peg_eval sexpPEG (print_sexp s ++ ls, pnt sxnt_sexp) =
+    peg_eval sexpPEG (print_sexp s ++ ls, pnt sxnt_sexp0 <~ rpt (tok isSpace ARB) (K ARB)))`,
+  strip_tac \\ simp[FUN_EQ_THM,pnt_def]
+  \\ Cases
+  >- (
+    simp[Once peg_eval_cases,FDOM_sexpPEG,sexpPEG_applied,ignoreR_def,peg_eval_seq_NONE,pnt_def]
+    \\ simp[Once peg_eval_cases,FDOM_sexpPEG,sexpPEG_applied,ignoreL_def,peg_eval_seq_NONE,peg_eval_rpt,PULL_EXISTS]
+    \\ rw[EQ_IMP_THM] \\ fs[pnt_def]
+    \\ metis_tac[peg_deterministic,peg_eval_list_isSpace_print_sexp,pairTheory.PAIR_EQ] )
+  \\ qmatch_goalsub_rename_tac`SOME p` \\ Cases_on`p`
+  \\ rw[Once peg_eval_cases,FDOM_sexpPEG,sexpPEG_applied,ignoreR_def,peg_eval_seq_SOME,pnt_def]
+  \\ simp[Once peg_eval_cases,FDOM_sexpPEG,sexpPEG_applied,ignoreL_def,peg_eval_seq_SOME,peg_eval_rpt,PULL_EXISTS]
+  \\ rw[EQ_IMP_THM] \\ fs[pnt_def,peg_eval_seq_SOME,peg_eval_rpt,PULL_EXISTS]
+  \\ metis_tac[peg_deterministic,peg_eval_list_isSpace_print_sexp,pairTheory.PAIR_EQ]);
+
+val nonStarter_def = Define`
+  (nonStarter #"." = T) ∧
+  (nonStarter #")" = T) ∧
+  (nonStarter #" " = T) ∧
+  (nonStarter _ = F)`;
+
+val peg_eval_sexp0_close = Q.store_thm("peg_eval_sexp0_close",
+  `nonStarter c ⇒ peg_eval sexpPEG (c::s,pnt sxnt_sexp0) NONE`,
+  rw[pnt_def,Once peg_eval_cases,FDOM_sexpPEG,sexpPEG_applied]
+  \\ rw[peg_eval_choicel_CONS,ignoreR_def,ignoreL_def,peg_eval_seq_NONE,pegf_def,tokeq_def,peg_eval_tok_NONE]
+  \\ rw[Once peg_eval_cases,FDOM_sexpPEG,sexpPEG_applied,pnt_def]
+  \\ rw[peg_eval_choicel_CONS,ignoreR_def,ignoreL_def,peg_eval_seq_NONE,pegf_def,tokeq_def,peg_eval_tok_NONE]
+  \\ rw[Once peg_eval_cases,FDOM_sexpPEG,sexpPEG_applied,pnt_def]
+  \\ rw[peg_eval_choicel_CONS,ignoreR_def,ignoreL_def,peg_eval_seq_NONE,pegf_def,tokeq_def,peg_eval_tok_NONE]
+  \\ fs[nonStarter_def]
+  \\ disj1_tac \\ EVAL_TAC);
+
+val peg_eval_sexpnum_nondigit = Q.store_thm("peg_eval_sexpnum_nondigit",
+  `¬isDigit c ⇒ peg_eval sexpPEG (c::cs,pnt sxnt_sexpnum) NONE`,
+  rw[pnt_def,Once peg_eval_cases,FDOM_sexpPEG,sexpPEG_applied,peg_eval_seq_NONE,pnt_def]
+  \\ disj1_tac
+  \\ rw[Once peg_eval_cases,FDOM_sexpPEG,sexpPEG_applied,peg_eval_tok_NONE])
+
+val peg_eval_sexp0_add_stop = Q.store_thm("peg_eval_sexp0_add_stop",
+  `peg_eval sexpPEG (str,pnt sxnt_sexp0) (SOME (r,s)) ⇒ nonStarter c ⇒
+   peg_eval sexpPEG (str++[c]++rst,pnt sxnt_sexp0) (SOME (r++[c]++rst,s))`,
+  simp[pnt_def,peg_eval_NT_SOME,FDOM_sexpPEG,sexpPEG_applied]
+  \\ cheat);
+
+val peg_eval_print_sexp0 = Q.store_thm("peg_eval_print_sexp0",
   `∀s. valid_sexp s ⇒
-       peg_eval sexpPEG (print_sexp s,sexpPEG.start) (SOME ("",s))`,
+     peg_eval sexpPEG (print_sexp s, pnt sxnt_sexp0) (SOME ("",s))`,
   ho_match_mp_tac(theorem"print_sexp_ind")
   \\ strip_tac >- (
     rw[print_sexp_def]
     \\ imp_res_tac peg_eval_valid_symbol
-    \\ fs[] )
+    \\ pop_assum mp_tac
+    \\ simp[pnt_def,Once peg_eval_NT_SOME,FDOM_sexpPEG,sexpPEG_applied,ignoreR_def,peg_eval_seq_SOME]
+    \\ simp[Once peg_eval_NT_SOME,FDOM_sexpPEG,sexpPEG_applied,ignoreL_def,peg_eval_seq_SOME,PULL_EXISTS]
+    \\ rpt strip_tac \\ fs[peg_eval_rpt] \\ rw[]
+    \\ imp_res_tac valid_symbol_no_spaces
+    \\ qspec_then`s`(mp_tac o Q.GEN`a`) (Q.ISPECL[`sexpPEG`,`isSpace`](Q.GENL[`P`,`G`]peg_eval_list_tok_nil))
+    \\ disch_then(qspec_then`ARB`mp_tac)
+    \\ impl_tac >- ( Cases_on`s` \\ fs[] )
+    \\ strip_tac
+    \\ imp_res_tac peg_deterministic \\ fs[] \\ rw[]
+    \\ imp_res_tac peg_eval_list_tok_imp_every
+    \\ rw[] \\ fs[] \\ rw[]
+    \\ imp_res_tac peg_eval_suffix
+    \\ fs[rich_listTheory.IS_SUFFIX_APPEND]
+    \\ rw[] \\ fs[]
+    \\ fs[listTheory.EVERY_MEM]
+    \\ Cases_on`l''`\\fs[pnt_def]
+    \\ metis_tac[] )
   \\ strip_tac >- (
     rw[print_sexp_def]
-    \\ MATCH_ACCEPT_TAC(SIMP_RULE(srw_ss())[]peg_eval_number))
+    \\ qspec_then`n`mp_tac peg_eval_number
+    \\ simp[pnt_def,Once peg_eval_NT_SOME,FDOM_sexpPEG,sexpPEG_applied,ignoreR_def,peg_eval_seq_SOME]
+    \\ simp[Once peg_eval_NT_SOME,FDOM_sexpPEG,sexpPEG_applied,ignoreL_def,peg_eval_seq_SOME,PULL_EXISTS]
+    \\ rpt strip_tac \\ fs[peg_eval_rpt] \\ rw[]
+    \\ qmatch_assum_rename_tac`peg_eval_list _ (toString n,_) (res,_)`
+    \\ `res = toString n`
+    by metis_tac[peg_eval_list_num_to_dec_string_no_spaces,peg_deterministic,pairTheory.PAIR_EQ]
+    \\ fs[pnt_def]
+    \\ imp_res_tac peg_eval_list_tok_imp_every
+    \\ imp_res_tac peg_eval_suffix
+    \\ fs[rich_listTheory.IS_SUFFIX_APPEND]
+    \\ rw[] \\ fs[]
+    \\ assume_tac EVERY_isDigit_num_to_dec_string
+    \\ rfs[listTheory.EVERY_MEM]
+    \\ Cases_on`i1`\\fs[]
+    \\ `∃h. isSpace h ∧ isDigit h` by metis_tac[]
+    \\ fs[stringTheory.isSpace_def,stringTheory.isDigit_def] )
   \\ strip_tac >- (
     rw[print_sexp_def]
-    \\ rw[pnt_def,peg_eval_NT_SOME,FDOM_sexpPEG,sexpPEG_applied]
-    \\ rw[ignoreR_def,peg_eval_seq_SOME,peg_eval_NT_SOME,FDOM_sexpPEG,sexpPEG_applied]
-    \\ qexists_tac`[]`
-    \\ rw[ignoreL_def,peg_eval_seq_SOME,peg_eval_rpt,PULL_EXISTS]
-    \\ rw[Once peg_eval_list,peg_eval_tok_NONE]
-    \\ srw_tac[boolSimps.DNF_ss][] \\ disj1_tac
-    \\ qexists_tac`[]`
-    \\ simp[peg_eval_list_tok_nil]
-    \\ conj_tac >- EVAL_TAC
-    \\ rw[pnt_def,peg_eval_NT_SOME,FDOM_sexpPEG,sexpPEG_applied]
-    \\ rw[peg_eval_choicel_CONS]
+    \\ simp[pnt_def,Once peg_eval_NT_SOME,FDOM_sexpPEG,sexpPEG_applied,ignoreR_def,peg_eval_seq_SOME]
+    \\ simp[peg_eval_choicel_CONS]
     \\ disj2_tac
     \\ conj_tac
     >- (
-      rw[Once peg_eval_cases,FDOM_sexpPEG,sexpPEG_applied,peg_eval_seq_NONE,pnt_def]
-      \\ disj1_tac
-      \\ rw[Once peg_eval_cases,FDOM_sexpPEG,sexpPEG_applied,peg_eval_tok_NONE]
+      simp[GSYM pnt_def]
+      \\ match_mp_tac peg_eval_sexpnum_nondigit
       \\ EVAL_TAC )
     \\ disj2_tac
     \\ conj_tac
@@ -345,44 +433,25 @@ val peg_eval_print_sexp = Q.prove(
     \\ first_assum(part_match_exists_tac(hd o strip_conj) o concl)
     \\ simp[rich_listTheory.FOLDR_MAP,destSXSYM_def]
     \\ srw_tac[boolSimps.ETA_ss][rich_listTheory.FOLDR_CONS_NIL] )
-  \\ rpt gen_tac \\ strip_tac
-  \\ simp[print_sexp_def]
-  \\ strip_tac
+  \\ rw[print_sexp_def]
   \\ BasicProvers.TOP_CASE_TAC \\ fs[] \\ rw[] \\ rfs[]
   >- (
     simp[pnt_def,peg_eval_NT_SOME,FDOM_sexpPEG,sexpPEG_applied]
-    \\ simp[ignoreR_def,peg_eval_seq_SOME]
-    \\ simp[peg_eval_NT_SOME,FDOM_sexpPEG,sexpPEG_applied]
-    \\ simp[ignoreL_def,peg_eval_seq_SOME,PULL_EXISTS]
-    \\ simp[peg_eval_rpt,PULL_EXISTS]
-    \\ simp[Once peg_eval_list,peg_eval_tok_NONE]
-    \\ srw_tac[boolSimps.DNF_ss][] \\ disj1_tac
-    \\ simp[pnt_def]
-    \\ simp[peg_eval_NT_SOME,FDOM_sexpPEG,sexpPEG_applied]
-    \\ simp[peg_eval_choicel_CONS,RIGHT_EXISTS_AND_THM]
-    \\ conj_tac >- EVAL_TAC
-    \\ srw_tac[boolSimps.DNF_ss][]
-    \\ disj2_tac \\ disj1_tac
-    \\ simp[pnt_def,ignoreL_def,peg_eval_seq_SOME,PULL_EXISTS,tokeq_def,peg_eval_tok_SOME]
+    \\ simp[peg_eval_choicel_CONS]
+    \\ disj2_tac
+    \\ conj_tac
+    >- (
+      simp[GSYM pnt_def]
+      \\ match_mp_tac peg_eval_sexpnum_nondigit
+      \\ EVAL_TAC )
+    \\ disj1_tac
+    \\ simp[ignoreL_def,peg_eval_seq_SOME,PULL_EXISTS,tokeq_def,peg_eval_tok_SOME]
     \\ simp[peg_eval_NT_SOME,FDOM_sexpPEG,sexpPEG_applied]
     \\ simp[peg_eval_choicel_CONS]
-    \\ rpt(qexists_tac`[]`)
-    \\ simp[peg_eval_list_tok_nil]
-    \\ conj_tac
-    >- (
-      simp[Once peg_eval_cases,FDOM_sexpPEG,sexpPEG_applied]
-      \\ simp[peg_eval_seq_NONE,pnt_def]
-      \\ disj1_tac
-      \\ simp[Once peg_eval_cases,FDOM_sexpPEG,sexpPEG_applied]
-      \\ simp[peg_eval_tok_NONE]
-      \\ EVAL_TAC )
-    \\ fs[Once strip_sxcons_def]
     \\ disj2_tac
-    \\ simp[pegf_def,peg_eval_seq_NONE,grabWS_def]
     \\ conj_tac
     >- (
-      simp[ignoreL_def,peg_eval_seq_NONE]
-      \\ simp[peg_eval_rpt,PULL_EXISTS]
+      simp[pegf_def,peg_eval_seq_NONE,grabWS_def,peg_eval_rpt,ignoreL_def,PULL_EXISTS]
       \\ REWRITE_TAC[GSYM listTheory.APPEND_ASSOC]
       \\ qmatch_goalsub_abbrev_tac`print_sexp s ++ ls`
       \\ qspecl_then[`s`,`ls`]mp_tac (GEN_ALL peg_eval_list_isSpace_print_sexp)
@@ -390,61 +459,197 @@ val peg_eval_print_sexp = Q.prove(
       \\ first_assum(part_match_exists_tac (hd o strip_conj) o concl) \\ simp[]
       \\ simp[tokeq_def,peg_eval_tok_NONE]
       \\ metis_tac[print_sexp_non_space,listTheory.APPEND])
-    \\ simp[peg_eval_seq_SOME,PULL_EXISTS,ignoreL_def]
-    \\ simp[peg_eval_rpt,PULL_EXISTS]
+    \\ simp[peg_eval_seq_SOME,PULL_EXISTS]
+    \\ simp[grabWS_def,ignoreL_def,peg_eval_seq_SOME,PULL_EXISTS,peg_eval_rpt]
     \\ REWRITE_TAC[GSYM listTheory.APPEND_ASSOC]
     \\ qmatch_goalsub_abbrev_tac`print_sexp s ++ ls`
     \\ qspecl_then[`s`,`ls`]mp_tac (GEN_ALL peg_eval_list_isSpace_print_sexp)
     \\ impl_tac \\ rw[]
     \\ first_assum(part_match_exists_tac (hd o strip_conj) o concl) \\ simp[]
-    \\ qpat_assum`peg_eval _ _ (_ (_,s))`mp_tac
-    \\ simp[pnt_def,Once peg_eval_NT_SOME,FDOM_sexpPEG,sexpPEG_applied,ignoreR_def]
-    \\ simp[peg_eval_seq_SOME,Once peg_eval_NT_SOME,FDOM_sexpPEG,sexpPEG_applied,ignoreL_def]
-    \\ simp[peg_eval_rpt,PULL_EXISTS]
-    \\ rpt gen_tac \\ strip_tac
-    \\ qmatch_assum_rename_tac`peg_eval_list _ (print_sexp _,_) (ps,ni)`
-    \\ `ps = print_sexp s ∧ ni = []`
-    by (
-      imp_res_tac print_sexp_non_space
-      \\ fs[Once peg_eval_list,peg_eval_tok_NONE,peg_eval_tok_SOME] )
-    \\ rpt var_eq_tac
-    \\ fs[pnt_def]
-    \\ cheat )
-  \\ BasicProvers.TOP_CASE_TAC \\ fs[] \\ rw[]
-  >- ( fs[Once strip_sxcons_def] )
-  \\ BasicProvers.TOP_CASE_TAC \\ rfs[]
-  >- (
-    rw[print_space_separated_def]
-    \\ rw[pnt_def,peg_eval_NT_SOME,FDOM_sexpPEG,sexpPEG_applied]
-    \\ simp[ignoreR_def,peg_eval_seq_SOME]
-    \\ rw[pnt_def,peg_eval_NT_SOME,FDOM_sexpPEG,sexpPEG_applied]
-    \\ simp[ignoreL_def,peg_eval_seq_SOME]
-    \\ fs[Once strip_sxcons_def]
-    \\ rpt var_eq_tac \\ rfs[]
-    \\ fs[Once strip_sxcons_def]
-    \\ every_case_tac \\ fs[]
-    \\ rpt var_eq_tac \\ rfs[] \\ rw[]
-    \\ simp[peg_eval_rpt,PULL_EXISTS]
-    \\ simp[peg_eval_NT_SOME,FDOM_sexpPEG,sexpPEG_applied]
-    \\ simp[peg_eval_choicel_CONS]
+    \\ last_assum(mp_tac o (MATCH_MP (GEN_ALL peg_eval_sexp0_add_stop)))
+    \\ disch_then(qspecl_then[`TL ls`,`HD ls`]mp_tac)
+    \\ simp[Abbr`ls`,nonStarter_def]
+    \\ strip_tac
+    \\ first_assum(part_match_exists_tac (hd o strip_conj) o concl) \\ simp[]
+    \\ simp[Once peg_eval_list]
     \\ srw_tac[boolSimps.DNF_ss][]
-    \\ disj2_tac \\ disj1_tac
-    \\ simp[Once peg_eval_list,peg_eval_tok_NONE,peg_eval_tok_SOME]
-    \\ simp[stringTheory.isSpace_def]
-    \\ simp[pnt_def]
-    \\ simp[Once peg_eval_cases,FDOM_sexpPEG,sexpPEG_applied]
-    \\ simp[peg_eval_seq_NONE,pnt_def]
-    \\ simp[Once peg_eval_cases,FDOM_sexpPEG,sexpPEG_applied]
-    \\ simp[peg_eval_tok_NONE]
-    \\ simp[stringTheory.isDigit_def]
-    \\ simp[ignoreL_def,peg_eval_seq_SOME,tokeq_def,peg_eval_tok_SOME]
+    \\ disj1_tac
+    \\ simp[peg_eval_seq_NONE,PULL_EXISTS,peg_eval_rpt]
+    \\ qpat_abbrev_tac`ls = #"."::_`
+    \\ qspec_then`ls`(mp_tac o Q.GEN`a`) (Q.ISPECL[`sexpPEG`,`isSpace`](Q.GENL[`P`,`G`]peg_eval_list_tok_nil))
+    \\ disch_then(qspec_then`ARB`mp_tac)
+    \\ impl_tac >- simp[Abbr`ls`,stringTheory.isSpace_def]
+    \\ strip_tac
+    \\ first_assum(part_match_exists_tac (hd o strip_conj) o concl) \\ simp[]
+    \\ simp[pnt_def,Once peg_eval_cases,FDOM_sexpPEG,sexpPEG_applied]
+    \\ simp[peg_eval_choicel_CONS,Abbr`ls`]
+    \\ simp[RIGHT_EXISTS_AND_THM]
+    \\ conj_tac
+    >- (
+      simp[tokeq_def,ignoreL_def,ignoreR_def,peg_eval_seq_NONE,peg_eval_tok_SOME,peg_eval_tok_NONE,pegf_def]
+      \\ simp[Once peg_eval_cases,FDOM_sexpPEG,sexpPEG_applied]
+      \\ simp[pnt_def,peg_eval_seq_NONE,peg_eval_tok_SOME,peg_eval_tok_NONE,pegf_def]
+      \\ simp[Once peg_eval_cases,FDOM_sexpPEG,sexpPEG_applied,peg_eval_tok_NONE]
+      \\ simp[stringTheory.isDigit_def]
+      \\ simp[Once peg_eval_cases,FDOM_sexpPEG,sexpPEG_applied]
+      \\ simp[pnt_def,peg_eval_seq_NONE,peg_eval_tok_SOME,peg_eval_tok_NONE,pegf_def])
+    \\ srw_tac[boolSimps.DNF_ss][]
+    \\ disj2_tac
+    \\ simp[pegf_def,peg_eval_seq_NONE,peg_eval_rpt,PULL_EXISTS]
+    \\ qpat_abbrev_tac`ls = #"."::_`
+    \\ qspec_then`ls`(mp_tac o Q.GEN`a`) (Q.ISPECL[`sexpPEG`,`isSpace`](Q.GENL[`P`,`G`]peg_eval_list_tok_nil))
+    \\ disch_then(qspec_then`ARB`mp_tac)
+    \\ impl_tac >- simp[Abbr`ls`,stringTheory.isSpace_def]
+    \\ strip_tac
+    \\ first_assum(part_match_exists_tac (hd o strip_conj) o concl) \\ simp[]
+    \\ simp[Abbr`ls`,peg_eval_tok_NONE,tokeq_def]
+    \\ simp[ignoreR_def,peg_eval_seq_SOME,PULL_EXISTS,peg_eval_rpt]
+    \\ qpat_abbrev_tac`ls = #"."::_`
+    \\ qspec_then`ls`(mp_tac o Q.GEN`a`) (Q.ISPECL[`sexpPEG`,`isSpace`](Q.GENL[`P`,`G`]peg_eval_list_tok_nil))
+    \\ disch_then(qspec_then`ARB`mp_tac)
+    \\ impl_tac >- simp[Abbr`ls`,stringTheory.isSpace_def]
+    \\ strip_tac
+    \\ first_assum(part_match_exists_tac (hd o strip_conj) o concl) \\ simp[]
+    \\ simp[Abbr`ls`,peg_eval_tok_SOME]
+    \\ first_assum(mp_tac o MATCH_MP (GEN_ALL peg_eval_list_isSpace_print_sexp))
+    \\ disch_then(qspec_then`")"`strip_assume_tac)
+    \\ first_assum(part_match_exists_tac (hd o strip_conj) o concl) \\ simp[]
+    \\ qpat_assum`_ _ _ (SOME (_,v1))`(mp_tac o (MATCH_MP (GEN_ALL peg_eval_sexp0_add_stop)))
+    \\ disch_then(qspecl_then[`""`,`#")"`]mp_tac)
+    \\ impl_tac >- simp[nonStarter_def]
+    \\ simp[pnt_def] \\ strip_tac
+    \\ first_assum(part_match_exists_tac (hd o strip_conj) o concl) \\ simp[]
+    \\ simp[replace_nil_def]
+    \\ metis_tac[peg_eval_list_tok_nil,EVAL``isSpace #")"``,listTheory.HD])
+  \\ BasicProvers.TOP_CASE_TAC \\ fs[]
+  >- ( fs[Once strip_sxcons_def] )
+  \\ BasicProvers.TOP_CASE_TAC \\ fs[]
+  >- (
+    fs[Once strip_sxcons_def]
+    \\ rw[] \\ rfs[]
+    \\ fs[Once strip_sxcons_def]
+    \\ every_case_tac \\ fs[] \\ rw[]
+    \\ rw[print_space_separated_def,pnt_def]
     \\ simp[peg_eval_NT_SOME,FDOM_sexpPEG,sexpPEG_applied]
     \\ simp[peg_eval_choicel_CONS]
-    \\ fs[pnt_def]
-    \\ simp[pegf_def,peg_eval_seq_SOME,peg_eval_seq_NONE,PULL_EXISTS]
-    \\ simp[grabWS_def,peg_eval_rpt,ignoreL_def,peg_eval_seq_NONE,PULL_EXISTS]
-    \\ cheat )
-  \\ cheat);
+    \\ disj2_tac
+    \\ conj_tac
+    >- (
+      simp[GSYM pnt_def]
+      \\ match_mp_tac peg_eval_sexpnum_nondigit
+      \\ EVAL_TAC )
+    \\ disj1_tac
+    \\ simp[ignoreL_def,peg_eval_seq_SOME,tokeq_def,peg_eval_tok_SOME]
+    \\ first_assum(mp_tac o (MATCH_MP (GEN_ALL peg_eval_sexp0_add_stop)))
+    \\ disch_then(qspecl_then[`""`,`#")"`]mp_tac)
+    \\ impl_tac >- EVAL_TAC
+    \\ rw[]
+    \\ simp[pnt_def]
+    \\ simp[peg_eval_NT_SOME,FDOM_sexpPEG,sexpPEG_applied]
+    \\ simp[peg_eval_choicel_CONS]
+    \\ disj2_tac
+    \\ conj_tac
+    >- (
+      simp[pegf_def,peg_eval_seq_NONE,grabWS_def,ignoreL_def,peg_eval_rpt,PULL_EXISTS]
+      \\ qspecl_then[`h`,`")"`]mp_tac (GEN_ALL peg_eval_list_isSpace_print_sexp)
+      \\ simp[] \\ strip_tac
+      \\ first_assum(part_match_exists_tac(hd o strip_conj) o concl) \\ simp[]
+      \\ simp[tokeq_def,peg_eval_tok_NONE]
+      \\ imp_res_tac print_sexp_non_space
+      \\ simp[])
+    \\ simp[peg_eval_seq_SOME,grabWS_def,ignoreL_def,peg_eval_rpt,PULL_EXISTS]
+    \\ qspecl_then[`h`,`")"`]mp_tac (GEN_ALL peg_eval_list_isSpace_print_sexp)
+    \\ simp[] \\ strip_tac
+    \\ first_assum(part_match_exists_tac(hd o strip_conj) o concl) \\ simp[]
+    \\ first_assum(part_match_exists_tac(hd o strip_conj) o concl) \\ simp[]
+    \\ simp[Once peg_eval_list]
+    \\ simp[peg_eval_seq_NONE,peg_eval_rpt,PULL_EXISTS]
+    \\ srw_tac[boolSimps.DNF_ss][]
+    \\ disj1_tac
+    \\ simp[replace_nil_def]
+    \\ qspec_then`")"`(mp_tac o Q.GEN`a`) (Q.ISPECL[`sexpPEG`,`isSpace`](Q.GENL[`P`,`G`]peg_eval_list_tok_nil))
+    \\ disch_then(qspec_then`ARB`mp_tac)
+    \\ impl_tac >- EVAL_TAC
+    \\ strip_tac
+    \\ first_assum(part_match_exists_tac(hd o strip_conj) o concl) \\ simp[]
+    \\ conj_tac >- (
+      match_mp_tac peg_eval_sexp0_close
+      \\ EVAL_TAC )
+    \\ rw[peg_eval_choicel_CONS]
+    \\ disj1_tac
+    \\ rw[pegf_def,peg_eval_seq_SOME,tokeq_def,peg_eval_tok_SOME,peg_eval_rpt]
+    \\ metis_tac[peg_eval_list_tok_nil,EVAL``isSpace(HD")")``] )
+  \\ BasicProvers.TOP_CASE_TAC \\ fs[]
+  >- (
+    fs[Once strip_sxcons_def]
+    \\ rw[] \\ fs[]
+    \\ fs[Once strip_sxcons_def]
+    \\ every_case_tac \\ fs[] \\ rw[]
+    \\ fs[Once strip_sxcons_def]
+    \\ every_case_tac \\ fs[] \\ rw[] \\ rfs[]
+    >- (
+      simp[pnt_def,peg_eval_NT_SOME,FDOM_sexpPEG,sexpPEG_applied]
+      \\ simp[peg_eval_choicel_CONS]
+      \\ disj2_tac
+      \\ conj_tac
+      >- (
+        simp[GSYM pnt_def]
+        \\ match_mp_tac peg_eval_sexpnum_nondigit
+        \\ EVAL_TAC )
+      \\ disj2_tac
+      \\ simp[ignoreR_def,ignoreL_def,peg_eval_seq_NONE,tokeq_def,peg_eval_tok_NONE,
+              peg_eval_seq_SOME,PULL_EXISTS,peg_eval_tok_SOME,pegf_def,grabWS_def,
+              peg_eval_rpt]
+      \\ disj1_tac
+      \\ fs[pnt_def]
+      \\ first_assum(part_match_exists_tac(last o strip_conj) o concl)
+      \\ simp[]
+      \\ metis_tac[peg_eval_list_isSpace_print_sexp,listTheory.APPEND_NIL] )
+    \\ simp[pnt_def,peg_eval_NT_SOME,FDOM_sexpPEG,sexpPEG_applied]
+    \\ simp[peg_eval_choicel_CONS]
+    \\ disj2_tac
+    \\ conj_tac
+    >- (
+      simp[GSYM pnt_def]
+      \\ match_mp_tac peg_eval_sexpnum_nondigit
+      \\ EVAL_TAC )
+    \\ disj1_tac
+    \\ simp[ignoreR_def,ignoreL_def,peg_eval_seq_NONE,tokeq_def,peg_eval_tok_NONE,
+            peg_eval_seq_SOME,PULL_EXISTS,peg_eval_tok_SOME,pegf_def,grabWS_def,
+            peg_eval_rpt]
+    \\ cheat (* see next one *))
+  \\ rw[]
+  \\ fs[Once strip_sxcons_def] \\ rw[]
+  \\ fs[Once strip_sxcons_def] \\ rw[]
+  \\ every_case_tac \\ fs[] \\ rw[]
+  \\ fs[Once strip_sxcons_def] \\ rw[]
+  \\ every_case_tac \\ fs[] \\ rw[]
+  \\ cheat (* similar to a few instances of previous cheat *));
+
+val peg_eval_print_sexp = Q.store_thm("peg_eval_print_sexp",
+  `∀s. valid_sexp s ⇒
+       peg_eval sexpPEG (print_sexp s,sexpPEG.start) (SOME ("",s))`,
+  rw[pnt_def,Once peg_eval_NT_SOME,FDOM_sexpPEG,sexpPEG_applied,ignoreR_def,
+     peg_eval_seq_SOME,peg_eval_rpt,ignoreL_def,PULL_EXISTS]
+  \\ rw[Once peg_eval_NT_SOME,FDOM_sexpPEG,sexpPEG_applied,ignoreL_def,
+        peg_eval_seq_SOME,peg_eval_rpt,PULL_EXISTS]
+  \\ imp_res_tac peg_eval_print_sexp0
+  \\ first_assum(part_match_exists_tac(el 2 o strip_conj) o concl)
+  \\ simp[]
+  \\ imp_res_tac (GEN_ALL peg_eval_list_isSpace_print_sexp)
+  \\ first_x_assum(qspec_then`[]`strip_assume_tac) \\ fs[]
+  \\ first_assum(part_match_exists_tac(hd o strip_conj) o concl)
+  \\ simp[]
+  \\ metis_tac[peg_eval_list_tok_nil]);
+
+val parse_print = Q.store_thm("parse_print",
+  `valid_sexp s ⇒ parse_sexp (print_sexp s) = SOME s`,
+  rw[parse_sexp_def,pairTheory.EXISTS_PROD]
+  \\ imp_res_tac peg_eval_print_sexp
+  \\ simp[pegparse_eq_SOME,wfG_sexpPEG]
+  \\ fs[]
+  \\ first_assum(part_match_exists_tac (hd o strip_conj) o concl)
+  \\ simp[]);
 
 (*
 val cs = listLib.list_compset()
@@ -456,20 +661,6 @@ val () = computeLib.add_thms[sexpPEG_exec_thm,pnt_def,ignoreR_def,ignoreL_def,to
   IF_CASES_TAC >- fs[stringTheory.isGraph_def] >>
   simp[choicel_def] >>
   CONV_TAC(computeLib.CBV_CONV cs) >> simp[] >>
-*)
-
-(*
-val parse_print = Q.store_thm("parse_print",
-  `parse_sexp (print_sexp s) = SOME s`,
-  rw[parse_sexp_def] >>
-  Cases_on`pegparse sexpPEG (print_sexp s)` >> simp[] >- (
-    imp_res_tac pegparse_eq_NONE >> fs[PEG_wellformed] >>
-    f"peg_eval"
-  reverse(Induct_on`s`)
-  >- (
-    rw[print_sexp_def] >>
-    rw[parse_sexp_def] >>
-    pegparse_eq_SOME
 *)
 
 val _ = export_theory()
